# Some Exercise

## Generics

### Functions

* Make CURRY function(2)
    - I : (A, B) => C
    - O : A => B => C 

    - signature : ((A, B) => C) => (A => B => C)


* Make CURRY function   
  - I : (A, B, C) => D   
  - O : A => B => C => D
   
  - Write signature:


* Make UN-CURRY function 
  - I : A => B => C => D  
  - O : (A, B, C) => D

  - Write signature:


* Make PARTIAL-APPLY function (tip : use Curry)
  - I : (A,B) => C , A
  - O : B => C

  - Write signature:

* Make SWAP function
  - I : (A,B) => C 
  - O : (B,A) => C

  - Write signature:


* Make COMBINE function
  - I : A => B, B => C
  - O : A => C

  - Write signature:

####  point-free combinator (SKI Combinator)
https://maartenfokkinga.github.io/utwente/mmf91m.pdf
https://wiki.haskell.org/Pointfree

* Make Identity Function (I)
  - signature : A => A

* Make Constant Function(K)
  - signature : A => B => A

* Make Apply Function(S)
  - signature : (A => (B => C)) => (A => B) => A => C // f(x)(g(x))

* Make Composition Function(B)
  - signature : (B => C) => (A => B) => A => C        // f(g(x))

* Make Flip-Argument Function(C)
  - signature : (A => B => C) => B => A => (B => A => C)

#### Make Y-Combinator Function(Y) ; fix 
  (higher-order function that allows a function that does not know its own name to call itself.)
  - https://stackoverflow.com/questions/34775656/explain-this-implementation-of-the-y-combinator-in-scala
  - https://antonkw.github.io/scala/y-combinator/
 
```scala

/**
 * <b>Fixed Point Combinator is:</b>
 * Y = λf.(λx.f (x x)) (λx.f (x x))
 *
 * <b>Proof of correctness:</b>
 * Y g  = (λf . (λx . f (x x)) (λx . f (x x))) g    (by definition of Y)
 * = (λx . g (x x)) (λx . g (x x))                  (β-reduction of λf: applied main function to g)
 * = (λy . g (y y)) (λx . g (x x))                  (α-conversion: renamed bound variable)
 * = g ((λx . g (x x)) (λx . g (x x)))              (β-reduction of λy: applied left function to right function)
 * = g (Y g)                                        (by second equality) [1]
 */
  
def Y[T](f: (T => T) => (T => T)): (T => T) = t => f(Y(f))(t) 

def fact = Y((f: Int => Int) => (n: Int) => if (n <= 0) 1 else n * f(n - 1))

println(fact(5));

```

#### Some practical

* Make Using-Resource function
  - signature :: (() => A) => (A => B) => B



### Data-Types

* Make Single-List

```scala

sealed trait SList[+A]
case class SCons[+A]( head: A, tail: SList[A]) extends SList[A]
case object SNil extends SList[Nothing]

val sl = SCons( 1, SCons(2, SNil));

```

* Make Binary Tree

```scala

sealed trait BTree[+A]
case class Branch[+A](left: Tree[A], right: Tree[A]) extends BTree[A]
case class Leaf[+A](value: A) extends BTree[A]
case object Nil extends BTree[Nothing]

val bt = Branch( Branch(Left(1), Leaf(2)), Nil)

```

* Make Maybe 

```scala
  ////////////////////////////////////////////////////////////////////////////////
  sealed trait Maybe[+A] {

    def flatMap[B]( f : A => Maybe[B]) = this match {
      case Just(a) => f(a)
      case Empty => Maybe.empty
    }

    def map[B]( f: A => B) = this match {
      case Just(a) => Just(f(a))
      case Empty => Maybe.empty
    }

    def map0[B](f : A => B) = flatMap( a => Maybe(f(a)))
    def map2[B](f : A => B) = flatMap( Maybe.apply[B] `@` f)   // point-free

  }

  case class Just[+A](get: A) extends Maybe[A]
  case object Empty extends Maybe[Nothing]

  ////////////////////////////////////////////////////////////////////////////////

  object Maybe {
    def apply[A](a : A): Maybe[A] = Just(a)
    def empty[A]: Maybe[A] = Empty
  }

  ////////////////////////////////////////////////////////////////////////////////
  val f0: Int => Maybe[Double] = ???
  val f1: Double => Maybe[String] = ???
  val f2: String => Maybe[Long] = ???
  val f3: Long => Maybe[Boolean] = ???

  val ret = (aa: Int) => for {
    a0 <- f0(aa)
    a1 <- f1(a0)
    a2 <- f2(a1)
    a3 <- f3(a2)
  } yield (a1, a3)

  implicit class FunctionWithComposePower[B,C]( f: B => C){
    def `@` [A]( g : A => B): A => C = a => f(g(a))
  }
```

#### Data Wrapping Function

* Make Function Wrapper
  - A => B
   
```scala
case class FunctionWrapper[A,B]( go: A => B)
```

* Make State Wrapper
  - S => (A, S)
   
```scala
case class StateWrapper[S,A]( go: S => (A, S))
```

* Make Read Wrapper
  - E => A
```scala
case class ReaderWrapper[E,A]( r: E => A)
```
