```scala
object FStructures {

  /**********************************************************************************
   *  
   */
  trait Functor[F[_]] { self =>

    def map[A,B](fa: F[A])(f: A => B): F[B]

    ////////////////////////////////////////////////////////////////////////////////

    def lift[A,B](f: A => B):F[A] => F[B] = fa => map(fa)(f)

    //////////////////////////////////////////////////
    def compose[G[_]: Functor] = new Functor[({type l[A] = F[G[A]]})#l] {

      val G = implicitly[Functor[G]]

      override def map[A, B](fga: F[G[A]])(f: A => B): F[G[B]] =
        self.map(fga)( G.lift(f))
    }
  }


  /**********************************************************************************
   *
   */
  trait Applicative[F[_]] extends Functor[F] { self =>

    def pure[A](a: A): F[A]
    def apply[A,B](fa: F[A])(ff: F[A => B]): F[B]

    ////////////////////////////////////////////////////////////////////////////////

    def map[A,B](fa: F[A])(f: A => B): F[B] = apply(fa)(pure(f))
    def flip[A,B](ff: F[A => B]): F[A] => F[B] = fa => apply(fa)(ff)

    def map2[A,B,C](fa: F[A], fb: F[B])(f: (A,B) => C): F[C] =
      apply(fa)(map(fb)( b => f(_, b)))

    

    //////////////////////////////////////////////////
    def compose[G[_]: Applicative]= new Applicative[({type l[A] = F[G[A]]})#l] {

      val G = implicitly[Applicative[G]]

      override def pure[A](a: A): F[G[A]] = self.pure( G.pure(a))

      override def apply[A, B](fga: F[G[A]])(fgf: F[G[A => B]]): F[G[B]] =
        self.apply(fga)( self.map(fgf)(G.flip) ) // F[G[A]] F[G[A] => G[B]]
    }

  }

  /**********************************************************************************
   *
   */
  trait Monad[F[_]] extends Applicative[F] {

    def flatMap[A,B](fa: F[A])(f: A => F[B]): F[B]

    ////////////////////////////////////////////////////////////////////////////////
    override def map[A, B](fa: F[A])(f: A => B): F[B] =
      flatMap(fa)(a => pure(f(a)))

    override def apply[A, B](fa: F[A])(ff: F[A => B]): F[B] =
      flatMap(fa)(a => map(ff)( _(a)))

  }

  /**********************************************************************************
   *
   */
  trait SemiGroup[A] {
    def combine( a0: A, a1: => A): A
  }

  trait SemiGroupK[F[_]] {
    def combine[A](a0: F[A], a1: F[A]): F[A]
  }

  /**********************************************************************************
   *
   */
  trait Monoid[A] extends SemiGroup[A]{
    def zero : A
  }

  /**********************************************************************************
   *
   */
  trait MonoidK[F[_]] extends SemiGroupK[F] { self =>

    def zero[A]: F[A]

    ////////////////////////////////////////////////////////////////////////////////
    def toMonoidFA[A] = new Monoid[F[A]] {
      override def zero: F[A] = self.zero
      override def combine(a0: F[A], a1: => F[A]): F[A] = self.combine(a0, a1)
    }
  }

  /**********************************************************************************
   *
   */
  object Monoid {

    def instance[A](zero0: A)(combine0: (A, =>A) => A)= new Monoid[A] {

      val z0 = zero0
      val c0 = combine0
      override def zero: A = z0
      override def combine(a0: A, a1: => A): A = c0(a0, a1)
    }
  }

  /**********************************************************************************
   *
   */
  trait Foldable[F[_]] { self =>

    def foldLeft[A,B](fa: F[A])(b: B)(f: ( B, A) => B): B
    def foldRight[A,B](fa: F[A])(b: B)(f: (A, B) => B): B

    ////////////////////////////////////////////////////////////////////////////////
    def foldMap[A,B: Monoid](fa: F[A])(f: A => B) = {
      val M = implicitly[Monoid[B]]
      foldLeft(fa)(M.zero)( (b, a) => M.combine(b, f(a)))
    }

    def fold[A:Monoid](fa: F[A]) =
      self.foldMap(fa)(identity)

    def foldK[G[_]: MonoidK, A](fga: F[G[A]]): G[A] = {
      val G = implicitly[MonoidK[G]]
      self.foldLeft(fga)(G.zero[A])((b, ga) => G.combine(b, ga))
    }

    //////////////////////////////////////////////////

    def compose[G[_]: Foldable] = new Foldable[({type l[A] = F[G[A]]})#l] {

      val G = implicitly[Foldable[G]]

      override def foldLeft[A, B](fga: F[G[A]])(b: B)(f: (B, A) => B): B =
        self.foldLeft(fga)(b)((b, ga) => G.foldLeft(ga)(b)(f))

      override def foldRight[A, B](fga: F[G[A]])(b: B)(f: (A, B) => B): B =
        self.foldRight(fga)(b)((ga, b) => G.foldRight(ga)(b)(f))
    }
  }

  /**********************************************************************************
   *
   */
  trait MonadFilter[F[_]] extends Monad[F]{ self =>
    def zero[A]: F[A]

    ////////////////////////////////////////////////////////////////////////////////
    def filter[A](fa: F[A])(p: A => Boolean): F[A] =
      self.flatMap(fa)(a => if(p(a)) pure(a) else zero )

    def filterM[A](fa: F[A])(p: A => F[Boolean]): F[A] =
      self.flatMap(fa)(a => flatMap(p(a))(b => if(b) pure(a) else zero) )
  }

  trait MonadCombine[F[_]] extends MonadFilter[F] with MonoidK[F]{

    def unite[G[_]: Foldable, A](fga: F[G[A]]): F[A] = {
      val G = implicitly[Foldable[G]]
      flatMap(fga)(ga => G.foldMap(ga)(a => pure(a))(toMonoidFA[A]))
    }
  }


  /**********************************************************************************
   *
   */
  trait Traverse[F[_]] extends Functor[F] with Foldable[F] {
    self =>

    def traverse[G[_] : Applicative, A, B](fa: F[A])(f: A => G[B]): G[F[B]]
  }

}
```
